Benchmarks/Dss/Cat/BiteCallFess.lean
@@ -3,6 +3,7 @@ import Benchmarks.Dss.Cat.Common
 open Solm ABI Ethereum Ethereum.EVM Reasoning.Theory Reasoning.Reach Reasoning.Refinement
 
 set_option maxRecDepth 2000000
+set_option maxHeartbeats 1000000
 
 namespace Benchmarks.Dss.Cat
 
